remove binder names in context declarations

theories/AutoSubst/PiUniv.sig
@@ -1,11 +1,10 @@
 sort : Type
-aname : Type
 term : Type
 
 tSort : sort -> term
 
-tProd : aname -> term -> (bind term in term) -> term
-tLambda : aname -> term -> (bind term in term) -> term
+tProd : term -> (bind term in term) -> term
+tLambda : term -> (bind term in term) -> term
 tApp : term -> term -> term
 
 tNat : term
