theories/Context.v
@@ -6,71 +6,19 @@ From LogRel Require Import Utils BasicAst.
 Set Primitive Projections.
 
 (** ** Context declaration *)
+(** Context: list of declarations *)
+(** Terms use de Bruijn indices to refer to context entries.*)
 
-(** The name is just a printing annotation: terms use de Bruijn indices to refer to context entries.*)
+Definition context := list term.
 
-Record context_decl := mkdecl {
-  decl_name : aname ;
-  decl_type : term
-}.
-
-Definition map_decl (f : term -> term) : context_decl -> context_decl :=
-  fun d => {| decl_name := d.(decl_name) ; decl_type := f d.(decl_type) |}.
-
-Lemma map_decl_id (f : term -> term) : f =1 id -> map_decl f =1 id.
-Proof.
-  intros Hf [a t].
-  cbv.
-  f_equal.
-  now apply Hf.
-Qed.
-
-Lemma compose_map_decl f g x :
-  map_decl f (map_decl g x) = map_decl (g >> f) x.
-Proof.
-  destruct x; reflexivity.
-Qed.
-
-Lemma map_decl_ext f g x : (forall x, f x = g x) -> map_decl f x = map_decl g x.
-Proof.
-  intros H; destruct x; rewrite /map_decl /=; f_equal; auto.
-Qed.
-
-#[global] Instance map_decl_proper : Proper (`=1` ==> Logic.eq ==> Logic.eq) map_decl.
-Proof.
-  intros f g Hfg x y ->. now apply map_decl_ext.
-Qed.
-
-#[global] Instance map_decl_pointwise : Proper (`=1` ==> `=1`) map_decl.
-Proof. intros f g Hfg x. rewrite /map_decl.
-  destruct x => /=. f_equal.
-  now rewrite Hfg.
-Qed.
-
-Arguments map_decl _ !_/.
-
-#[global] Instance Ren_decl : (Ren1 (nat -> nat) context_decl context_decl) :=
-  fun ρ t => map_decl (ren_term ρ) t.
-
-Arguments Ren_decl _ !_/.
-
-Ltac fold_ren_decl := change Ren_decl with ren1 in *.
-Smpl Add fold_ren_decl : refold.
-
-Definition vass a A := {| decl_name := a ; decl_type := A |}.
-
-(** ** Context: list of declarations *)
-
-Definition context := list context_decl.
-
-Notation "'ε'" := (@nil context_decl).
-Notation " Γ ,, d " := (@cons context_decl d Γ) (at level 20, d at next level).
-Notation " Γ ,,, Δ " := (@app context_decl Δ Γ) (at level 25, Δ at next level, left associativity).
+Notation "'ε'" := (@nil term).
+Notation " Γ ,, d " := (@cons term d Γ) (at level 20, d at next level).
+Notation " Γ ,,, Δ " := (@app term Δ Γ) (at level 25, Δ at next level, left associativity).
 
 (** States that a definition, correctly weakened, is in a context. *)
-Inductive in_ctx : context -> nat -> context_decl -> Type :=
+Inductive in_ctx : context -> nat -> term -> Type :=
   | in_here (Γ : context) d : in_ctx (Γ,,d) 0 (d⟨↑⟩)
-  | in_there (Γ : context) d d' n : in_ctx Γ n d -> in_ctx (Γ,,d') (S n) (map_decl (ren_term shift) d).
+  | in_there (Γ : context) d d' n : in_ctx Γ n d -> in_ctx (Γ,,d') (S n) (ren_term shift d).
 
 Lemma in_ctx_inj Γ n decl decl' :
   in_ctx Γ n decl -> in_ctx Γ n decl' -> decl = decl'.
