theories/LogicalRelation/NormalRed.v
@@ -10,30 +10,29 @@ Context `{GenericTypingProperties}.
 
 Set Printing Primitive Projection Parameters.
 
-Program Definition normRedΠ0 {Γ nF F G l} (h : [Γ ||-Π<l> tProd nF F G])
-  : [Γ ||-Π<l> tProd nF F G] :=
-  {| PiRedTyPack.na := nF ; 
-     PiRedTyPack.dom := F ;
+Program Definition normRedΠ0 {Γ F G l} (h : [Γ ||-Π<l> tProd F G])
+  : [Γ ||-Π<l> tProd F G] :=
+  {| PiRedTyPack.dom := F ;
      PiRedTyPack.cod := G |}.
 Solve All Obligations with 
   intros;
-  assert (wΠ : whnf (tProd nF F G)) by constructor;
+  assert (wΠ : whnf (tProd F G)) by constructor;
   pose proof (e := redtywf_whnf (PiRedTyPack.red h) wΠ);
   symmetry in e; injection e; clear e; 
-  destruct h as [??????? domRed codRed codExt] ; 
+  destruct h as [?????? domRed codRed codExt] ; 
   intros; cbn in *; subst; eassumption + now eapply domRed + 
   (unshelve eapply codRed ; tea ; irrelevance)
   + ( irrelevance0; [reflexivity| unshelve eapply codExt; tea]; irrelevance).
 
-Definition normRedΠ {Γ nF F G l} (h : [Γ ||-<l> tProd nF F G])
-  : [Γ ||-<l> tProd nF F G] :=
+Definition normRedΠ {Γ F G l} (h : [Γ ||-<l> tProd F G])
+  : [Γ ||-<l> tProd F G] :=
   LRPi' (normRedΠ0 (invLRΠ h)).
 
 #[program]
-Definition normLambda {Γ nF F nF' F' G t l RΠ} 
-  (Rlam : [Γ ||-<l> tLambda nF' F' t : tProd nF F G | normRedΠ RΠ ]) :
-  [Γ ||-<l> tLambda nF' F' t : tProd nF F G | normRedΠ RΠ ] :=
-  {| PiRedTm.nf := tLambda nF' F' t |}.
+Definition normLambda {Γ F F' G t l RΠ} 
+  (Rlam : [Γ ||-<l> tLambda F' t : tProd F G | normRedΠ RΠ ]) :
+  [Γ ||-<l> tLambda F' t : tProd F G | normRedΠ RΠ ] :=
+  {| PiRedTm.nf := tLambda F' t |}.
 Solve All Obligations with
   intros;
   pose proof (e := redtmwf_whnf (PiRedTm.red Rlam) whnf_tLambda);
