theories/Substitution/Introductions/Lambda.v
@@ -16,29 +16,29 @@ Context `{GenericTypingProperties}.
 
 
 
-Context {Γ nF F G l} {VΓ : [||-v Γ]} (VF : [Γ ||-v<l> F | VΓ]) 
-  (VΓF := validSnoc nF VΓ VF)
-  (VG : [Γ ,, vass nF F ||-v<l> G | VΓF])
+Context {Γ F G l} {VΓ : [||-v Γ]} (VF : [Γ ||-v<l> F | VΓ]) 
+  (VΓF := validSnoc VΓ VF)
+  (VG : [Γ ,, F ||-v<l> G | VΓF])
   (VΠFG := PiValid VΓ VF VG).
 
 
-Lemma consWkEq {Δ Ξ} σ (ρ : Δ ≤ Ξ) a Z : Z[up_term_term σ]⟨wk_up nF F[σ] ρ⟩[a..] = Z[a .: σ⟨ρ⟩].
+Lemma consWkEq {Δ Ξ} σ (ρ : Δ ≤ Ξ) a Z : Z[up_term_term σ]⟨wk_up F[σ] ρ⟩[a..] = Z[a .: σ⟨ρ⟩].
 Proof. bsimpl; cbn; now rewrite rinstInst'_term_pointwise. Qed.
 
 Lemma consWkEq' {Δ Ξ} σ (ρ : Δ ≤ Ξ) a Z : Z[up_term_term σ][a .: ρ >> tRel] = Z[a .: σ⟨ρ⟩].
 Proof. bsimpl; cbn; now rewrite rinstInst'_term_pointwise. Qed.
 
-Lemma lamBetaRed {t} (Vt : [Γ ,, vass nF F ||-v<l> t : G | VΓF | VG]) 
+Lemma lamBetaRed {t} (Vt : [Γ ,, F ||-v<l> t : G | VΓF | VG]) 
   {Δ σ} (wfΔ : [ |-[ ta ] Δ]) (Vσ : [VΓ | Δ ||-v σ : Γ | wfΔ]) 
   {Δ0 a} (ρ : Δ0 ≤ Δ) (wfΔ0 : [|-Δ0])
   (RFσ : [Δ0 ||-<l> F[σ]⟨ρ⟩]) 
   (ha : [RFσ | _ ||- a : _])
   (RGσ : [Δ0 ||-<l> G[up_term_term σ][a .: ρ >> tRel]]) :
-    [_ ||-<l> tApp (tLambda nF F t)[σ]⟨ρ⟩ a : _ | RGσ] × 
-    [_ ||-<l> tApp (tLambda nF F t)[σ]⟨ρ⟩ a ≅ t[a .: σ⟨ρ⟩] : _ | RGσ].
+    [_ ||-<l> tApp (tLambda F t)[σ]⟨ρ⟩ a : _ | RGσ] × 
+    [_ ||-<l> tApp (tLambda F t)[σ]⟨ρ⟩ a ≅ t[a .: σ⟨ρ⟩] : _ | RGσ].
 Proof.
-  pose proof (Vσa := consWkSubstS nF VF ρ wfΔ0 Vσ ha); instValid Vσa.
-  pose proof (VσUp :=  liftSubstS' nF VF Vσ).
+  pose proof (Vσa := consWkSubstS VF ρ wfΔ0 Vσ ha); instValid Vσa.
+  pose proof (VσUp :=  liftSubstS' VF Vσ).
   instValid Vσ. instValid VσUp.  escape.
   irrelevance0. 1: now rewrite consWkEq'.
   eapply redwfSubstTerm; tea.
@@ -49,13 +49,13 @@ Proof.
   eapply wfc_cons; tea; eapply wft_wk; tea.
 Qed.
 
-Lemma betaValid {t a} (Vt : [Γ ,, vass nF F ||-v<l> t : G | VΓF | VG]) 
+Lemma betaValid {t a} (Vt : [Γ ,, F ||-v<l> t : G | VΓF | VG]) 
   (Va : [Γ ||-v<l> a : F | VΓ | VF]) :
-  [Γ ||-v<l> tApp (tLambda nF F t) a ≅ t[a..] : G[a..] | VΓ | substS nF VG Va].
+  [Γ ||-v<l> tApp (tLambda F t) a ≅ t[a..] : G[a..] | VΓ | substS VG Va].
 Proof.
   constructor; intros. instValid Vσ.
-  pose (Vσa := consSubstS (nA := nF) _ _ Vσ _ RVa). instValid Vσa.
-  pose proof (VσUp :=  liftSubstS' nF VF Vσ).
+  pose (Vσa := consSubstS _ _ Vσ _ RVa). instValid Vσa.
+  pose proof (VσUp :=  liftSubstS' VF Vσ).
   instValid Vσ. instValid VσUp.  escape.
   assert (eq : forall t, t[a..][σ] = t[up_term_term σ][a[σ]..]) by (intros; now bsimpl).
   assert (eq' : forall t, t[a..][σ] = t[a[σ].: σ]) by (intros; now bsimpl).
@@ -68,16 +68,16 @@ Proof.
     Unshelve. 2:rewrite <- eq; now rewrite eq'.
 Qed.
 
-Lemma lamValid0 {t} (Vt : [Γ ,, vass nF F ||-v<l> t : G | VΓF | VG]) 
+Lemma lamValid0 {t} (Vt : [Γ ,, F ||-v<l> t : G | VΓF | VG]) 
   {Δ σ} (wfΔ : [ |-[ ta ] Δ]) (Vσ : [VΓ | Δ ||-v σ : Γ | wfΔ]) :
-  [validTy VΠFG wfΔ Vσ | Δ ||- (tLambda nF F t)[σ] : (tProd nF F G)[σ]].
+  [validTy VΠFG wfΔ Vσ | Δ ||- (tLambda F t)[σ] : (tProd F G)[σ]].
 Proof.
-  pose proof (VσUp :=  liftSubstS' nF VF Vσ).
+  pose proof (VσUp :=  liftSubstS' VF Vσ).
   instValid Vσ. instValid VσUp. escape.
   pose (RΠ := normRedΠ RVΠFG); refold.
-  enough [RΠ | Δ ||- (tLambda nF F t)[σ] : (tProd nF F G)[σ]] by irrelevance.
-  assert [Δ |- (tLambda nF F t)[σ] : (tProd nF F G)[σ]] by (escape; cbn; gen_typing).
-  exists (tLambda nF F t)[σ]; intros; cbn in *.
+  enough [RΠ | Δ ||- (tLambda F t)[σ] : (tProd F G)[σ]] by irrelevance.
+  assert [Δ |- (tLambda F t)[σ] : (tProd F G)[σ]] by (escape; cbn; gen_typing).
+  exists (tLambda F t)[σ]; intros; cbn in *.
   + now eapply redtmwf_refl.
   + constructor.
   + apply tm_nf_lam.
@@ -87,7 +87,7 @@ Proof.
     1,2: now constructor.
     assert (eqσ : forall Z, Z[up_term_term σ] = Z[up_term_term σ]⟨upRen_term_term S⟩[(tRel 0) ..])
     by (intro; bsimpl; cbn; now rewrite rinstInst'_term_pointwise).
-    assert [Δ,, vass nF F[σ] |-[ ta ] tApp (tLambda nF F[σ] t[up_term_term σ])⟨S⟩ (tRel 0) ⇒*  t[up_term_term σ]⟨upRen_term_term S⟩[(tRel 0)..] : G[up_term_term σ]].
+    assert [Δ,, F[σ] |-[ ta ] tApp (tLambda F[σ] t[up_term_term σ])⟨S⟩ (tRel 0) ⇒*  t[up_term_term σ]⟨upRen_term_term S⟩[(tRel 0)..] : G[up_term_term σ]].
     {
       rewrite (eqσ G). eapply redtm_beta.
       * renToWk; eapply wft_wk; tea; gen_typing.
@@ -99,8 +99,8 @@ Proof.
     1: now eapply redty_refl.
     rewrite <- (eqσ t); eapply escapeEqTerm; now eapply LREqTermRefl_.
   + eapply lamBetaRed; tea. 
-  + pose proof (Vσa := consWkSubstS nF VF ρ h Vσ ha).
-    pose proof (Vσb := consWkSubstS nF VF ρ h Vσ hb).
+  + pose proof (Vσa := consWkSubstS VF ρ h Vσ ha).
+    pose proof (Vσb := consWkSubstS VF ρ h Vσ hb).
     assert (Vσab : [_ ||-v _ ≅ (b .: σ⟨ρ⟩) : _ | _ | _ | Vσa]).
     1:{
       unshelve eapply consSubstSEq'.
@@ -118,25 +118,25 @@ Proof.
       irrelevance. now rewrite consWkEq'.
 Qed.
 
-Lemma lamValid {t} (Vt : [Γ ,, vass nF F ||-v<l> t : G | VΓF | VG])
+Lemma lamValid {t} (Vt : [Γ ,, F ||-v<l> t : G | VΓF | VG])
    :
-    [Γ ||-v<l> tLambda nF F t : tProd nF F G | VΓ | VΠFG ].
+    [Γ ||-v<l> tLambda F t : tProd F G | VΓ | VΠFG ].
 Proof.
   opector. 1: now apply lamValid0.
   intros.
-  pose (VσUp :=  liftSubstS' nF VF Vσ).
-  pose proof (VσUp' :=  liftSubstS' nF VF Vσ').
-  pose proof (VσUprea :=  liftSubstSrealign' nF VF Vσσ' Vσ').
-  pose proof (VσσUp := liftSubstSEq' nF VF Vσσ').
+  pose (VσUp :=  liftSubstS' VF Vσ).
+  pose proof (VσUp' :=  liftSubstS' VF Vσ').
+  pose proof (VσUprea :=  liftSubstSrealign' VF Vσσ' Vσ').
+  pose proof (VσσUp := liftSubstSEq' VF Vσσ').
   instAllValid Vσ Vσ' Vσσ';  instValid VσUp'; instAllValid VσUp VσUprea VσσUp.
   pose (RΠ := normRedΠ RVΠFG); refold.
-  enough [RΠ | Δ ||- (tLambda nF F t)[σ] ≅ (tLambda nF F t)[σ'] : (tProd nF F G)[σ]] by irrelevance.
+  enough [RΠ | Δ ||- (tLambda F t)[σ] ≅ (tLambda F t)[σ'] : (tProd F G)[σ]] by irrelevance.
   unshelve econstructor.
-  - change [RΠ | Δ ||- (tLambda nF F t)[σ] : (tProd nF F G)[σ]].
+  - change [RΠ | Δ ||- (tLambda F t)[σ] : (tProd F G)[σ]].
     eapply normLambda.
     epose (lamValid0 Vt wfΔ Vσ).
     irrelevance.
-  - change [RΠ | Δ ||- (tLambda nF F t)[σ'] : (tProd nF F G)[σ]].
+  - change [RΠ | Δ ||- (tLambda F t)[σ'] : (tProd F G)[σ]].
     eapply normLambda.
     eapply LRTmRedConv.
     2: epose (lamValid0 Vt wfΔ Vσ'); irrelevance.
@@ -169,14 +169,14 @@ Proof.
         set (x := ren_term _ _); change x with (t[up_term_term σ']⟨upRen_term_term S⟩); clear x.
         do 2 rewrite <- eqσ ; eapply escapeEqTerm; now eapply validTmExt.
   - refold; cbn; intros.
-    pose proof (Vσa := consWkSubstS nF VF ρ h Vσ ha).
+    pose proof (Vσa := consWkSubstS VF ρ h Vσ ha).
     assert (ha' : [ _||-<l> a : _| wk ρ h RVF0]).
     1: {
       eapply LRTmRedConv; tea.
       irrelevance0; [reflexivity|].
       eapply wkEq; eapply (validTyExt VF); tea.
     }
-    pose proof (Vσa' := consWkSubstS nF VF ρ h Vσ' ha').
+    pose proof (Vσa' := consWkSubstS VF ρ h Vσ' ha').
     assert (Vσσa : [_ ||-v _ ≅ (a .: σ'⟨ρ⟩) : _ | _ | _ | Vσa]).
     {
       unshelve eapply consSubstSEq'.
@@ -195,21 +195,21 @@ Qed.
 
 
 
-Lemma ηeqEqTermConvNf {σ Δ f} (ρ := @wk1 Γ nF F)
+Lemma ηeqEqTermConvNf {σ Δ f} (ρ := @wk1 Γ F)
   (wfΔ : [|- Δ]) (Vσ : [Δ ||-v σ : Γ | VΓ| wfΔ])
   (RΠFG := normRedΠ (validTy VΠFG wfΔ Vσ))
-  (Rf : [Δ ||-<l> f[σ] : (tProd nF F G)[σ] | RΠFG ]) :
-  [Δ ,, vass nF F[σ] |- tApp f⟨ρ⟩[up_term_term σ] (tRel 0) ≅ tApp (PiRedTm.nf Rf)⟨↑⟩ (tRel 0) : G[up_term_term σ]].
+  (Rf : [Δ ||-<l> f[σ] : (tProd F G)[σ] | RΠFG ]) :
+  [Δ ,, F[σ] |- tApp f⟨ρ⟩[up_term_term σ] (tRel 0) ≅ tApp (PiRedTm.nf Rf)⟨↑⟩ (tRel 0) : G[up_term_term σ]].
 Proof.
   refold.
-  pose (VσUp :=  liftSubstS' nF VF Vσ).
+  pose (VσUp :=  liftSubstS' VF Vσ).
   instValid Vσ; instValid VσUp; escape.
   destruct (PiRedTm.red Rf); cbn in *.
-  assert (wfΔF : [|- Δ,, vass nF F[σ]]) by gen_typing.
-  unshelve epose proof (r := PiRedTm.app Rf (@wk1 Δ nF F[σ]) wfΔF (var0 _ _ _ _)).
+  assert (wfΔF : [|- Δ,, F[σ]]) by gen_typing.
+  unshelve epose proof (r := PiRedTm.app Rf (@wk1 Δ F[σ]) wfΔF (var0 _ _ _)).
   1: now rewrite wk1_ren_on.
   assumption.
-  assert (eqσ : forall σ Z, Z[up_term_term σ] = Z[up_term_term σ][(tRel 0) .: @wk1 Δ nF F[σ] >> tRel])
+  assert (eqσ : forall σ Z, Z[up_term_term σ] = Z[up_term_term σ][(tRel 0) .: @wk1 Δ F[σ] >> tRel])
   by (intros; bsimpl; cbn; now rewrite rinstInst'_term_pointwise).
   eapply convtm_exp. 
   1: now eapply redty_refl.
@@ -218,32 +218,32 @@ Proof.
     1: eapply redtm_app.
     2: eapply (ty_var wfΔF (in_here _ _)).
     1:{
-      replace (f⟨_⟩[_]) with f[σ]⟨@wk1 Δ nF F[σ]⟩ by (unfold ρ; now bsimpl).
+      replace (f⟨_⟩[_]) with f[σ]⟨@wk1 Δ F[σ]⟩ by (unfold ρ; now bsimpl).
       eapply redtm_meta_conv. 3: reflexivity.
       1: eapply redtm_wk; tea.
       now rewrite wk1_ren_on.
     }
     fold ren_term. rewrite eqσ; now bsimpl. 
-  * rewrite <- (wk1_ren_on Δ nF F[σ]); unshelve eapply redtmwf_refl.
+  * rewrite <- (wk1_ren_on Δ F[σ]); unshelve eapply redtmwf_refl.
     rewrite eqσ; eapply escapeTerm ; irrelevance.
     Unshelve. 2,4: rewrite <- eqσ; tea.
 Qed.
 
 
-Lemma ηeqEqTerm {σ Δ f g} (ρ := @wk1 Γ nF F)
-  (Vfg : [Γ ,, vass nF F ||-v<l> tApp f⟨ρ⟩ (tRel 0) ≅ tApp g⟨ρ⟩ (tRel 0) : G | VΓF | VG ])
+Lemma ηeqEqTerm {σ Δ f g} (ρ := @wk1 Γ F)
+  (Vfg : [Γ ,, F ||-v<l> tApp f⟨ρ⟩ (tRel 0) ≅ tApp g⟨ρ⟩ (tRel 0) : G | VΓF | VG ])
   (wfΔ : [|- Δ]) (Vσ : [Δ ||-v σ : Γ | VΓ| wfΔ])
   (RΠFG := validTy VΠFG wfΔ Vσ)
-  (Rf : [Δ ||-<l> f[σ] : (tProd nF F G)[σ] | RΠFG ])
-  (Rg : [Δ ||-<l> g[σ] : (tProd nF F G)[σ] | RΠFG ]) :
-  [Δ ||-<l> f[σ] ≅ g[σ] : (tProd nF F G)[σ] | RΠFG ].
+  (Rf : [Δ ||-<l> f[σ] : (tProd F G)[σ] | RΠFG ])
+  (Rg : [Δ ||-<l> g[σ] : (tProd F G)[σ] | RΠFG ]) :
+  [Δ ||-<l> f[σ] ≅ g[σ] : (tProd F G)[σ] | RΠFG ].
 Proof.
   set (RΠ := normRedΠ RΠFG); refold.
-  enough [Δ ||-<l> f[σ] ≅ g[σ] : (tProd nF F G)[σ] | RΠ ] by irrelevance.
+  enough [Δ ||-<l> f[σ] ≅ g[σ] : (tProd F G)[σ] | RΠ ] by irrelevance.
   opector.
-  - change [Δ ||-<l> f[σ] : (tProd nF F G)[σ] | RΠ ]; irrelevance.
-  - change [Δ ||-<l> g[σ] : (tProd nF F G)[σ] | RΠ ]; irrelevance.
-  - cbn; pose (VσUp :=  liftSubstS' nF VF Vσ).
+  - change [Δ ||-<l> f[σ] : (tProd F G)[σ] | RΠ ]; irrelevance.
+  - change [Δ ||-<l> g[σ] : (tProd F G)[σ] | RΠ ]; irrelevance.
+  - cbn; pose (VσUp :=  liftSubstS' VF Vσ).
     instValid Vσ; instValid VσUp; escape.
     destruct (PiRedTm.red p); destruct (PiRedTm.red p0); cbn in *.
     eapply convtm_eta; tea.
@@ -251,9 +251,9 @@ Proof.
     etransitivity ; [symmetry| etransitivity]; tea; eapply ηeqEqTermConvNf.
   - cbn; intros.
     set (ν := (a .: σ⟨ρ0⟩)).
-    pose (Vν := consWkSubstS nF VF ρ0 h Vσ ha).
+    pose (Vν := consWkSubstS VF ρ0 h Vσ ha).
     instValid Vσ; instValid Vν; escape.
-    assert (wfΔF : [|- Δ,, vass nF F[σ]]) by gen_typing.
+    assert (wfΔF : [|- Δ,, F[σ]]) by gen_typing.
     cbn in *.
     assert (eq : forall t, t⟨ρ⟩[a .: σ⟨ρ0⟩] = t[σ]⟨ρ0⟩) by (intros; unfold ρ; now bsimpl).
     do 2 rewrite eq in RVfg.
@@ -271,11 +271,11 @@ Proof.
       now bsimpl.
 Qed.
 
-Lemma etaeqValid {f g} (ρ := @wk1 Γ nF F)
-  (Vf : [Γ ||-v<l> f : tProd nF F G | VΓ | VΠFG ])
-  (Vg : [Γ ||-v<l> g : tProd nF F G | VΓ | VΠFG ]) 
-  (Vfg : [Γ ,, vass nF F ||-v<l> tApp f⟨ρ⟩ (tRel 0) ≅ tApp g⟨ρ⟩ (tRel 0) : G | VΓF | VG ]) :
-  [Γ ||-v<l> f ≅ g : tProd nF F G | VΓ | VΠFG].
+Lemma etaeqValid {f g} (ρ := @wk1 Γ F)
+  (Vf : [Γ ||-v<l> f : tProd F G | VΓ | VΠFG ])
+  (Vg : [Γ ||-v<l> g : tProd F G | VΓ | VΠFG ]) 
+  (Vfg : [Γ ,, F ||-v<l> tApp f⟨ρ⟩ (tRel 0) ≅ tApp g⟨ρ⟩ (tRel 0) : G | VΓF | VG ]) :
+  [Γ ||-v<l> f ≅ g : tProd F G | VΓ | VΠFG].
 Proof.
   constructor; intros ??? Vσ; instValid Vσ; now eapply ηeqEqTerm.
 Qed.
